Add Desc and SmartDesc for Expressions

Katydid/Expr/Desc.lean
@@ -1,3 +1,4 @@
+import Std.Data.List.Lemmas
 import Std.Classes.Order
 
 /-
@@ -8,12 +9,19 @@ We represent the description (including AST) of the expr, or as we call it the D
 
 inductive Desc where
   | intro
-    (name : String)
-    (hash : UInt64)
-    (params : List Desc)
+    (name: String)
+    (params: List Desc)
+    (hash: UInt64)
     (reader: Bool)
-  : Desc
   deriving Repr
+
+def Desc.name (desc: Desc): String :=
+  match desc with
+  | ⟨ name, _, _, _ ⟩ => name
+
+def Desc.params (desc: Desc): List Desc :=
+  match desc with
+  | ⟨ _, params, _, _⟩ => params
 
 /-
 The `hash` field is important, because it is used to efficiently compare functions calls, so that we can reorder and simplify.  For example:
@@ -21,50 +29,167 @@ The `hash` field is important, because it is used to efficiently compare functio
   * and(lt(3, 5), lt(3, 5)) => lt(3, 5)
   * or(and(lt(3, 5), contains("abcd", "bc")), and(contains("abcd", "bc"), lt(3, 5))) => and(contains("abcd", "bc"), lt(3, 5))
 -/
-
-/- The reader field tells us whether the function has any variables or can be evaluated at compile time. -/
-
-def get_reader (desc: Desc): Bool :=
-  match desc with
-  | ⟨ _, _, _, reader⟩ => reader
-
-def get_hash (desc: Desc): UInt64 :=
-  match desc with
-  | ⟨ _, hash, _, _ ⟩ => hash
-
 def hash_list (innit: UInt64) (list: List UInt64): UInt64 :=
   List.foldl (fun acc h => 31 * acc + h) innit list
 
 def hash_string (s: String): UInt64 :=
   hash_list 0 (List.map (Nat.toUInt64 ∘ Char.toNat) (String.toList s))
 
-def hash_with_name (name: String) (params: List Desc): UInt64 :=
-  hash_list (31 * 17 + hash_string name) (List.map get_hash params)
+def hash_desc (desc: Desc): UInt64 :=
+  match desc with
+  | ⟨ name, params, _, _⟩ => hash_list (31 * 17 + hash_string name) (hash_params params)
+where hash_params (params: List Desc): List UInt64 :=
+  match params with
+  | [] => []
+  | param::params => hash_desc param :: hash_params params
 
-#eval hash_string "abcdefghjasdfasdf"
+def Desc.hash (desc: Desc): UInt64 :=
+  hash_desc desc
 
-def introDesc (name: String) (params: List Desc): Desc :=
-  Desc.intro
-    name
-    (hash_with_name name params)
-    params
-    (List.any params get_reader)
+def any_reader (d: Desc): Bool :=
+  match d with
+  | ⟨ _, params, _, _⟩ => any_params params
+where any_params (params: List Desc): Bool :=
+  match params with
+  | [] => false
+  | param::params => any_reader param || any_params params
 
-#eval introDesc "a" List.nil
+/- The reader field tells us whether the function has any variables or can be evaluated at compile time. -/
+def Desc.reader (desc: Desc): Bool :=
+  any_reader desc
 
-def introReaderDesc (name: String) (params: List Desc): Desc :=
-  ⟨
-    name,
-    hash_with_name name params,
-    params,
-    true
-  ⟩
+inductive IsSmart : Desc → Prop
+  | isSmart: ∀
+    (name: String)
+    (params: List Desc)
+    (hash: UInt64)
+    (reader: Bool),
+    desc = Desc.intro name params hash reader
+    → hash = desc.hash
+    → reader = desc.reader
+    → (∀ param, param ∈ params → IsSmart param)
+    → IsSmart desc
 
-def cmp (x y: Desc): Ordering :=
+structure SmartDesc where
+  subtype: { desc: Desc // IsSmart desc }
+
+def SmartDesc.name (d: SmartDesc): String :=
+  d.subtype.val.name
+
+def IsSmartParams (params: List Desc): Prop := ∀ param, param ∈ params → IsSmart param
+
+def conj_is_smart_params {p: Desc} {ps: List Desc} (isSmart: IsSmartParams (p :: ps)):
+  IsSmart p /\ IsSmartParams ps :=
+  ⟨ isSmart p (List.mem_cons_self _ _), λ p' h => isSmart p' (List.mem_cons_of_mem _ h) ⟩
+
+def cons_is_smart_params (sx: IsSmart x) (sxs: IsSmartParams xs): IsSmartParams (x :: xs) := by
+  unfold IsSmartParams
+  intro x' inxs
+  cases inxs with
+  | head => exact sx
+  | tail _ inxs =>
+    unfold IsSmartParams at sxs
+    apply sxs
+    exact inxs
+
+def SmartParams := {params: List Desc // IsSmartParams params}
+
+def empty_smart_params: SmartParams := ⟨[], λ p h => False.elim (List.not_mem_nil p h)⟩
+
+def cons_smart_params (sx: SmartDesc) (sxs: SmartParams): SmartParams :=
+  match sx.subtype with
+  | ⟨ x, xIsSmart ⟩ =>
+    match sxs with
+    | ⟨ xs, xsIsSmart ⟩ =>
+      ⟨ x :: xs , cons_is_smart_params xIsSmart xsIsSmart ⟩
+
+def sparams_to_list (params: List Desc) (isSmartParams: IsSmartParams params): List SmartDesc := by
+  cases params with
+  | nil => exact []
+  | cons p ps =>
+    cases conj_is_smart_params isSmartParams with
+    | intro pIsSmart psIsSmart =>
+      exact ⟨p, pIsSmart⟩ :: sparams_to_list ps psIsSmart
+
+def list_to_sparams (sdecs: List SmartDesc): SmartParams :=
+  match sdecs with
+  | [] => empty_smart_params
+  | x::xs => cons_smart_params x (list_to_sparams xs)
+
+def SmartDesc.params (s: SmartDesc): List SmartDesc := by
+  cases s.subtype with
+  | mk desc isSmart =>
+    refine sparams_to_list desc.params ?_
+    cases isSmart with
+    | isSmart _ params _ _ descEq _ _ isSmartParams =>
+      rw [descEq]
+      exact isSmartParams
+
+inductive Forall {α : Type u} (p : α → Prop) : List α → Prop
+  | nil  : Forall p ([] : List α)
+  | cons : ∀ {x xs}, p x → Forall p xs → Forall p (x :: xs)
+
+def forall_sparams (params: List Desc) (sparams: IsSmartParams params): Forall IsSmart params :=
+  match params with
+  | [] => Forall.nil
+  | _p::ps =>
+    let sparams' := conj_is_smart_params sparams
+    Forall.cons sparams'.left (forall_sparams ps sparams'.right)
+
+def SmartDesc.hash (d: SmartDesc): UInt64 :=
+  -- The hash has been precalculated, so we don't need to recompute it.
+  match d.subtype.val with
+  | ⟨ _, _, hash, _⟩ => hash
+
+def SmartDesc.reader (d: SmartDesc): Bool :=
+  -- The reader has been precalculated, so we don't need to recompute it.
+  match d.subtype.val with
+  | ⟨ _, _, _, reader⟩ => reader
+
+def hash_with_sparams (name: String) (sparams: List SmartDesc): UInt64 :=
+  hash_list (31 * 17 + hash_string name) (List.map SmartDesc.hash sparams)
+
+def SmartDesc.intro_func (name: String) (sparams: List SmartDesc): SmartDesc :=
+  let params := List.map (λ s => s.subtype.val) sparams
+  let hash := hash_with_sparams name sparams
+  let reader := List.any params Desc.reader
+  let desc := Desc.intro name params hash reader
+  by
+     refine ⟨ desc, IsSmart.isSmart name params hash reader ?_ ?_ ?_ ?_ ⟩
+     · rfl
+     · sorry -- TODO
+     · sorry -- TODO
+     · sorry -- TODO
+
+def SmartDesc.intro_var (name: String): SmartDesc :=
+  let params := []
+  let hash := hash_with_sparams name []
+  let reader := true
+  let desc := Desc.intro name params hash reader
+  by
+     refine ⟨ desc, IsSmart.isSmart name params hash reader ?_ ?_ ?_ ?_ ⟩
+     · rfl
+     · sorry -- TODO
+     · sorry -- TODO
+     · sorry -- TODO
+
+def SmartDesc.intro_const (name: String): SmartDesc :=
+  let params := []
+  let hash := hash_with_sparams name []
+  let reader := false
+  let desc := Desc.intro name params hash reader
+  by
+     refine ⟨ desc, IsSmart.isSmart name params hash reader ?_ ?_ ?_ ?_ ⟩
+     · rfl
+     · sorry -- TODO
+     · sorry -- TODO
+     · sorry -- TODO
+
+private def cmp' (x y: Desc): Ordering :=
   match x with
-  | ⟨xname, xhash, xparams, _⟩ =>
+  | ⟨xname, xparams, xhash, _⟩ =>
     match y with
-    | ⟨yname, yhash, yparams, _⟩ =>
+    | ⟨yname, yparams, yhash, _⟩ =>
       let chash := compare xhash yhash
       if chash != Ordering.eq
       then chash
@@ -72,26 +197,35 @@ def cmp (x y: Desc): Ordering :=
         let cname := compare xname yname
         if cname != Ordering.eq
         then cname
-        else cmps xparams yparams
-where cmps (xs ys : List Desc) : Ordering :=
+        else cmps' xparams yparams
+where cmps' (xs ys : List Desc) : Ordering :=
   match xs, ys with
   | x::xs, y::ys =>
-    let r := cmp x y
+    let r := cmp' x y
     if r != Ordering.eq
     then r
-    else cmps xs ys
+    else cmps' xs ys
   | _, _ => Ordering.eq
 
-instance : Hashable Desc where
-  hash x := get_hash x
+def cmp (x y: SmartDesc): Ordering :=
+  match x with
+  | ⟨xdesc, _ ⟩ =>
+    match y with
+    | ⟨ydesc, _ ⟩ =>
+      cmp' xdesc ydesc
 
-instance : Ord Desc where
-  compare x y := cmp x y
+instance : Hashable SmartDesc where
+  hash x := x.hash
 
-theorem cmp_symm : ∀ (x y : Desc),
-  Ordering.swap (cmp x y) = cmp y x := by
+def SmartDesc.compare := cmp
+
+instance : Ord SmartDesc where
+  compare x y := x.compare y
+
+theorem cmp_symm : ∀ (x y : SmartDesc),
+  Ordering.swap (x.compare y) = y.compare x := by
   -- TODO
   sorry
 
-instance : Std.OrientedCmp cmp where
+instance : Std.OrientedCmp SmartDesc.compare where
   symm x y := cmp_symm x y
